Added fibonacci program for specific inputs

examples/sum_to_10.v
@@ -11,11 +11,11 @@ Import InstructionSetNotation.
 Check CHIP8InitialStateEmptyRam.
 
 Definition sum_to_10 :=
-  ( ( v1 := n0 ::: n1 ) ;; (*counter : n0*)
+  ( ( v1 := n0 ::: n0 ) ;; (*counter : n0*)
     ( v2 := n0 ::: na ) ;; (*sum to 10 : n2*)
     ( v3 := n0 ::: n0 ) ;; (*sum : n4*)
-    ( v3 :=+ v1 ) ;; (*add v1 to v3 : n6*)
     ( v1 :=+ n0 ::: n1 ) ;; (*update counter*)
+    ( v3 :=+ v1 ) ;; (*add v1 to v3 : n6*)
     ( skip if v1 equal to v2 ) ;;
     ( jump to n2 ::: n0 ::: n6 ) ;;
     ( ret ) (*exit?*)
@@ -24,10 +24,8 @@ Definition sum_to_10 :=
 Definition CHIP_prog prog :=
   updateRam (prog 512 init_memory) CHIP8InitialStateEmptyRam.
 
-Compute (nth 1 (exec_step (CHIP_prog sum_to_10) 14).(registers) x00).
-
 Example sum_to_10_prog :
-      (nth 1 (exec_step (CHIP_prog sum_to_10) 14).(registers) x00) = x04.
+      (nth 3 (exec_step (CHIP_prog sum_to_10) 41).(registers) x00) = x37.
 Proof.
   reflexivity.
 Qed.
