examples/fibonacci.v
@@ -1,0 +1,66 @@
+Require Import Coq.Init.Byte Coq.Strings.Byte.
+From CHIP8 Require Import InstructionSet.
+From CHIP8 Require Import HelperDataTypes.
+From CHIP8 Require Import MainMemory.
+From CHIP8 Require Import MainSystem.
+
+Require Import Coq.Lists.List.
+Require Import Coq.micromega.Lia.
+
+Import InstructionSetNotation.
+
+Fixpoint fibonacci_aux a b c :=
+  match c with
+  | 0 => a
+  | S c' => fibonacci_aux (b) (a+b) c'
+  end.
+
+Fixpoint fibonacci n :=
+  fibonacci_aux 0 1 n.
+
+Definition fibonacci_n_chip8 n :=
+  ( ( v1 := n0 ::: n0 ) ;; (*value of a : n0*)
+    ( v2 := n0 ::: n1 ) ;; (*value of b : n2*)
+    ( v3 := n0 ::: n ) ;; (*value to reach : n4*)
+    ( v4 := n0 ::: n0 ) ;; (*value of counter : n6*)
+    (* Start of program *)
+    ( skip if v4 equal to v3 ) (*if equal go to end : n8*) ;;
+    ( jump to n2 ::: n0 ::: ne ) (* jump to procedure : na*) ;;
+    ( ret ) (* return point : nc *) ;;
+    ( v4 :=+ n0 ::: n1 ) ;;
+    ( v5 := v2 ) ;;
+    ( v2 :=+ v1 ) ;;
+    ( v1 := v5) ;; 
+    ( jump to n2 ::: n0 ::: n8 ) 
+  ).
+
+Definition CHIP_prog prog :=
+  updateRam (prog 512 init_memory) CHIP8InitialStateEmptyRam.
+
+Example sum_to_10_prog : forall n,
+    fibonacci (n_to_nat n) < 256 -> 
+    Some (nth 1 (exec_step (CHIP_prog (fibonacci_n_chip8 n)) 2000).(registers) x00)
+    =
+    of_nat (fibonacci (n_to_nat n)).
+Proof.
+  intros n. intro H ; destruct n eqn:E.
+  + reflexivity.
+  + reflexivity.
+  + reflexivity.
+  + reflexivity.
+  + reflexivity.
+  + reflexivity.
+  + reflexivity.
+  + reflexivity.
+  + reflexivity.
+  + reflexivity.
+  + reflexivity.
+  + reflexivity.
+  + reflexivity.
+  + reflexivity.
+  + simpl in H. lia.
+  + simpl in H. lia.
+Qed.
+
+
+
